nontotal

src/pca.lean
@@ -4,22 +4,24 @@ import tactic
 universe variable u
 variables {α : Type u}
 
-class partial_magma (α : Type u) :=
+class pmagma (α : Type u) :=
 (mul : α → α → option α)
-infixl ` ⬝ ` := partial_magma.mul
+infixl ` ⬝ ` := pmagma.mul
 infix ` ↓= `:50 := λ x y, x = some y
 prefix `↓`:80 := some
 
 abbreviation defined : option α → bool := option.is_some
-def partial_magma.mmul [partial_magma α] : option α → option α → option α
+abbreviation udefined : option α → bool := option.is_none
+
+def pmagma.mmul [pmagma α] : option α → option α → option α
 | ↓x ↓y := x ⬝ y
 | _ _   := none
-instance pm_mul [partial_magma α] : has_mul (option α) := {mul := @partial_magma.mmul α _}
+instance pm_mul [pmagma α] : has_mul (option α) := {mul := @pmagma.mmul α _}
 
-@[simp] lemma partial_magma.none_l [partial_magma α] (p : option α) : none * p = none := option.cases_on p rfl (λ a, rfl)
-@[simp] lemma partial_magma.none_r [partial_magma α] (p : option α) : p * none = none := option.cases_on p rfl (λ a, rfl)
+@[simp] lemma pmagma.none_l [pmagma α] (p : option α) : none * p = none := option.cases_on p rfl (λ _, rfl)
+@[simp] lemma pmagma.none_r [pmagma α] (p : option α) : p * none = none := option.cases_on p rfl (λ _, rfl)
 
-lemma defined_l [partial_magma α] {p q : option α} : defined (p * q) → defined p :=
+lemma defined_l [pmagma α] {p q : option α} : defined (p * q) → defined p :=
 begin
   contrapose,
   assume (h0 : ¬ defined p),
@@ -28,7 +30,7 @@ begin
   simp,
 end
 
-lemma defined_r [partial_magma α] {p q : option α} : defined (p * q) → defined q :=
+lemma defined_r [pmagma α] {p q : option α} : defined (p * q) → defined q :=
 begin
   contrapose,
   assume (h0 : ¬ defined q),
@@ -37,37 +39,45 @@ begin
   simp,
 end
 
-def tot [partial_magma α] (a : α) : Prop := ∀ x : α, defined (↓a * ↓x) = tt
+def tot [pmagma α] (a : α) : Prop := ∀ x : α, defined (↓a * ↓x) = tt
 
-def partial_magma.equiv [partial_magma α] (a b : option α) : Prop := ∀ x : α, a * ↓x = b * ↓x
-infix ` ≃ `:50 := partial_magma.equiv
+def pmagma.equiv [pmagma α] (a b : option α) : Prop := ∀ x : α, a * ↓x = b * ↓x
+infix ` ≃ `:50 := pmagma.equiv
 
-@[refl] lemma partial_magma.refl [partial_magma α] (a : option α) : a ≃ a := λ x, rfl
+@[refl] lemma pmagma.refl [pmagma α] (a : option α) : a ≃ a := λ x, rfl
 
-@[trans] lemma partial_magma.trans [partial_magma α] (a b c : option α) (eab : a ≃ b) (ebc : b ≃ c) : a ≃ c :=
+@[trans] lemma pmagma.trans [pmagma α] (a b c : option α) (eab : a ≃ b) (ebc : b ≃ c) : a ≃ c :=
 by { intros x, rw (eab x), exact ebc x, }
 
+class nontotal (α : Type u) [pmagma α] :=
+(p q : α)
+(undefined : p ⬝ q = none)
+
+@[simp] lemma nontototal_simp [pmagma α] [nontotal α] : (↓nontotal.p * ↓nontotal.q : option α) = none := nontotal.undefined
 
 /- Partial Combinatory Algebra -/
-class pca (α : Type u) extends partial_magma α :=
+class pca (α : Type u) extends pmagma α :=
 (k : α)
-(ktot : ∀ x, defined (k ⬝ x))
 (k_constant : ∀ x y : α, k ⬝ x * y = x)
 (s : α)
-(stot' : ∀ x y : α, defined (s ⬝ x * y))
+(s_defined : ∀ x y : α, defined (s ⬝ x * y))
 (s_substitution : ∀ x y z : α, s ⬝ x * y * z = (x ⬝ z) * (y ⬝ z))
-
 
 namespace pca
 
 variables [pca α]
 
+lemma ktot : tot (k : α) :=
+by { intros x, have h : defined (k ⬝ x * x) = tt, { rw k_constant x x, refl, }, exact defined_l h, }
+
+lemma stot : tot (s : α) := λ a, defined_l (s_defined a a)
+
 def const (x : α) : α := option.get (ktot x)
-def subst (x y : α) : α := option.get (stot' x y)
+def subst (x y : α) : α := option.get (s_defined x y)
 notation `𝐤` := const
 notation `𝐬` := subst
 
-@[simp] lemma k_simp (a : α) : ↓k * ↓a = ↓(𝐤 a) := by { unfold const, simp, refl }
+@[simp] lemma k_simp (a : α) : ↓k * ↓a = ↓(𝐤 a) := by { unfold const, simp, }
 @[simp] lemma s_simp (a b : α) : ↓s * ↓a * ↓b = ↓(𝐬 a b) := by { unfold subst, simp, refl }
 @[simp] lemma k_simp0 (a b : α) : ↓(𝐤 a) * ↓b = ↓a := by { rw ← k_simp, exact k_constant _ _, }
 @[simp] lemma s_simp0 (a b c : α) : ↓(𝐬 a b) * ↓c = (↓a * ↓c) * (↓b * ↓c) := by { rw ← s_simp, exact s_substitution _ _ _, }
@@ -76,94 +86,7 @@ def i : α := 𝐬 k k
 @[simp] lemma i_ident (a : α) : ↓i * ↓a = ↓a := by { unfold i, simp, }
 lemma itot : tot (i : α) := by { intros x, simp, refl, }
 
-lemma stot : tot (s : α) := λ a, defined_l (stot' a a)
-
 def subst' (x : α) : α := option.get (stot x)
 notation `𝐬'` := subst'
-
-inductive lambda (α : Type u)
-| var : ℕ → lambda
-| com : α → lambda
-| app : lambda → lambda → lambda
-prefix `#` := lambda.var
-prefix `&`:max := lambda.com
-instance lambda_mul (α : Type u) : has_mul (lambda α) := ⟨lambda.app⟩
-
-def lam (n : ℕ) :lambda α → lambda α
-| #m := if n = m then &i else &k * #m
-| &c := &k * &c
-| (l * k) := &s * (lam l) * (lam k)
-notation `Λ`x`,` := lam x 
-
-def expr : lambda α → option α
-| #x := ↓k
-| &c := ↓c
-| (l * k) := (expr l) * (expr k)
-
-lemma lambda_defined (n : ℕ) : ∀ (e : lambda α), defined (expr (Λ n, e) : option α)
-| #e := begin
-    cases (eq.decidable n e),
-    { simp[lam, expr, if_neg h], exact rfl, },
-    { simp[lam, expr, if_pos h], exact rfl, },
-  end
-| &c := ktot c
-| (l * m) := begin
-    simp [lam, expr], 
-    let a := option.get (lambda_defined l),
-    let b := option.get (lambda_defined m),
-    have ha : expr (Λ n, l) = ↓a, { simp },
-    have hb : expr (Λ n, m) = ↓b, { simp },
-    rw [ha, hb],
-    exact stot' a b
-  end
-
-notation n` ↦ `l := option.get (lambda_defined n l)
-
-namespace recursion
-
-def d : α := 0 ↦ Λ 1, (#0 * #0 * #1)
-def dd : lambda α := Λ 0, (Λ 1, (#0 * #0 * #1))
-
-lemma dtot (f : α) : defined (d ⬝ f) :=
-by { change (d ⬝ f) with (↓d * ↓f), unfold d, simp [lam, expr], exact rfl, }
-
-lemma diagonal (f x : α) : d ⬝ f * x = f ⬝ f * x :=
-begin
-  calc
-    d ⬝ f * ↓x = ↓d * ↓f * ↓x : rfl
-    ...        = f ⬝ f * ↓x   : by { unfold d, simp [lam, expr], refl, }
-end
-
-def v : α := 0 ↦ Λ 1, (#0 * (&d * #1))
-def n : α := 0 ↦ &d * (&v * #0)
-
-theorem recursion (f : α) : n ⬝ f ≃ f * (n ⬝ f) :=
-begin
-  intros x,
-  let vf := (0 ↦ &f * (&d * #0)),  
-  have hv : ↓v * ↓f = ↓vf, { unfold v, simp [lam, expr], },
-  have nf_dvf : ↓n * ↓f = ↓d * ↓vf,  { unfold n, unfold v, simp [lam, expr], },
-  calc
-    n ⬝ f * x = ↓n * ↓f * x         : rfl
-    ...       = ↓d * ↓vf * x        : by { rw nf_dvf, }
-    ...       = ↓vf * ↓vf * x       : diagonal vf x
-    ...       = ↓f * (↓d * ↓vf) * x : by { simp [lam, expr], }
-    ...       = ↓f * (↓n * ↓f) * x  : by { rw nf_dvf, }
-end
-
-theorem ntot (f : α) : defined (↓n * ↓f) :=
-begin
-  let vf := (0 ↦ &f * (&d * #0)),  
-  have hv : ↓v * ↓f = ↓vf, { unfold v, simp [lam, expr], },
-  have nf_dvf : ↓n * ↓f = ↓d * ↓vf,  { unfold n, unfold v, simp [lam, expr], },
-  rw nf_dvf,
-  exact (dtot _)
-end
-
-end recursion
-
-def fixpoint : α := recursion.n
-def recursion  (f x : α) : ↓fixpoint * ↓f * ↓x = f * (↓fixpoint * ↓f) * ↓x := recursion.recursion f x
-def fixpoint_of (f : α) : α := option.get (recursion.ntot f)
 
 end pca
